Pretty much how stuff was when I came back to it

src/Core.Environment.fst
@@ -1,5 +1,6 @@
 module Core.Environment
 
+open Core.Weaken
 open Core.Name
 open Core.Ltt
 
@@ -12,59 +13,27 @@ unopteq type local_env (tm:list local_name -> Type) : (vars:list local_name) -> 
             -> name:local_name // the name bound by the binder
             -> local_env tm vars
             -> local_env tm (name :: vars)
-private val shave_vars : n:local_name
-                       -> l:list local_name{n `List.mem` l}
-                       -> Tot (list local_name)
-let rec shave_vars n (x::xs) =
-  if n = x then xs else shave_vars n xs
 
-(*private val expand_term : #vars:list local_name
-                        -> #outer:list local_name
-                        -> raw_term vars
-                        -> Tot (raw_term (vars @ outer))
-let expand_term #vars #outer #tm = function
-  | RVar fc n -> RVar fc n
-  | RUniverse fc -> RUniverse fc
-  | RAbs fc var bnd body -> RAbs fc var bnd body
-  | RApp fc l r -> RApp fc l r
-
-
-type expand_tm (tm:list local_name -> Type) =
-  vars:list local_name -> name:local_name ->
-  tm vars -> Tot (tm (name :: vars))
-
-private val expand_binder : #tm:(list local_name -> Type)
-                          -> #vars:list local_name
-                          -> name:local_name
-                          -> tm_helper:expand_tm tm
-                          -> binder (tm vars)
-                          -> Tot (binder (tm (name :: vars)))
-let expand_binder #tm #vars name tm_helper = map_binder (tm_helper vars name)*)
-
-val env_lookup : #tm:(list local_name -> Type)
-               -> #vars:list local_name
-               -> name:local_name
-               -> local_env tm vars
-               -> Tot (
-               option (if name `List.mem` vars
-                       then (binder (tm (shave_vars name vars)))
-                       else False))
-let rec env_lookup #tm #vars name envr =
-  match envr with
+let rec env_lookup
+  (#vars:list local_name)
+  (tm:list local_name -> Type)
+  [|weaken tm|]
+  (name:local_name)
+  (envr:local_env tm vars)
+  : option (binder (tm vars))
+  = match envr with
   | EmptyEnv -> None
   | ConsEnv bnd n' rest ->
-    if n' = name then (
-      Some bnd
-    ) else (
-      env_lookup name rest
-    )
-
-(*val env_lookup_lemma : #tm:(list local_name -> Type)
-                     -> #vars:list local_name
-                     -> name:local_name
-                     -> envr:local_env tm vars
-                     -> Lemma
-  (ensures (let res = env_lookup name envr in
-           Some? res ==> (name `List.mem` vars /\ res `has_type` binder (tm (shave_vars name vars)))))
-let env_lookup_lemma #tm #vars name envr = ()*)
-
+    let opt_bnd = if n' = name
+      then Some bnd
+      else env_lookup tm name rest in
+    let v :: vs = vars in
+    assert (opt_bnd `has_type` option (binder (tm vs)));
+    let map_bnd (bnd:binder (tm vs))
+      : binder (tm vars) =
+      let bnd' = weaken' #vs #v (binder_tm tm) bnd in
+      assert (bnd' `has_type` binder (tm vars));
+      bnd' in
+    match opt_bnd with
+    | Some b -> Some (map_bnd b)
+    | None -> None
