src/Core.Weaken.fst
@@ -1,0 +1,24 @@
+module Core.Weaken
+
+open Core.Name
+
+class weaken tm = {
+  weaken_ns' : vars:list local_name -> ns:list local_name -> tm vars -> Tot (tm (ns @ vars))
+}
+
+let weaken_ns
+  (#vars:list local_name)
+  (tm:list local_name -> Type)
+  [|d:weaken tm|]
+  (ns:list local_name)
+  (t:tm vars)
+  = weaken_ns' #tm vars ns t
+
+let weaken'
+  (#vars:list local_name)
+  (#name:local_name)
+  (tm:list local_name -> Type)
+  [|d:weaken tm|]
+  (t:tm vars)
+  : tm (name :: vars)
+  = weaken_ns' #tm vars [name] t
